fix sorries and start adding heaplang

Coinductive/CoInd.lean
@@ -210,15 +210,19 @@ theorem cofix_eq {α} (f : α → F α) a :
     . rfl
     simp [cofix, CoInd.fold, cofix_approx]
 
-def CoInd.le.bot [Inhabited (F PUnit)] : CoInd F :=
+section partial_order
+open Lean.Order
+open Classical
+
+def CoInd.bot [Inhabited (F PUnit)] : CoInd F :=
   cofix F (λ _ : PUnit => default) ⟨⟩
 
-theorem CoInd.le.bot_eq [Inhabited (F PUnit)] :
+theorem CoInd.bot_eq [Inhabited (F PUnit)] :
   bot F = CoInd.fold F (QPF.map F (λ _ : PUnit => bot F) default) :=
     by unfold bot; rw (occs := [1]) [cofix_eq]
 
 def CoInd.le [Inhabited (F PUnit)] (c1 : CoInd F) (c2 : CoInd F) : Prop :=
-  c1 = le.bot F ∨ coherent1 CoInd.le (QPF.unpack c1.unfold) (QPF.unpack c2.unfold)
+  c1 = bot F ∨ coherent1 CoInd.le (QPF.unpack c1.unfold) (QPF.unpack c2.unfold)
 coinductive_fixpoint monotonicity fun f f' himp => by
   rintro _ _ (⟨⟨⟩⟩|x)
   . simp
@@ -231,10 +235,10 @@ theorem CoInd.le.coherent_bot_eq  [Inhabited (F PUnit)] c :
     intro h
     ext n
     induction n generalizing c h; rfl
-    rw [CoInd.le.bot_eq]
+    rw [CoInd.bot_eq]
     rw [<-unfold_fold _ c, CoInd.fold_approx]
     simp [CoInd.fold_approx]
-    rw [CoInd.le.bot_eq] at h
+    rw [CoInd.bot_eq] at h
     simp at h
     split at h
     rcases h
@@ -244,22 +248,20 @@ theorem CoInd.le.coherent_bot_eq  [Inhabited (F PUnit)] c :
     subst_eqs
     grind [le, QPF.map]
 
-theorem CoInd.le.rfl [Inhabited (F PUnit)] c:
-  CoInd.le F c c := by
+instance [Inhabited (F PUnit)] : PartialOrder (CoInd F) where
+  rel := CoInd.le F
+  rel_refl := by
+    intro c
     apply CoInd.le.coinduct _ (Eq)
     case x => grind
     intro x1 x2 h
     subst_eqs
     right
-    rcases (QPF.unpack (unfold F x1)) with ⟨_, _⟩ <;> try trivial
+    rcases (QPF.unpack (CoInd.unfold F x1)) with ⟨_, _⟩ <;> try trivial
     constructor <;> try trivial
     simp
-
-theorem CoInd.le.trans [Inhabited (F PUnit)] c1 c2 c3:
-  CoInd.le F c1 c2 →
-  CoInd.le F c2 c3 →
-  CoInd.le F c1 c3 := by
-    intro _ _
+  rel_trans := by
+    intro c1 c2 c3 _ _
     apply CoInd.le.coinduct _ (λ c1 c3 => ∃ c2, CoInd.le F c1 c2 ∧ CoInd.le F c2 c3)
     case x => grind
     rintro c1 c3 ⟨c2, h1, h2⟩
@@ -279,12 +281,8 @@ theorem CoInd.le.trans [Inhabited (F PUnit)] c1 c2 c3:
     subst_eqs
     constructor <;> try rfl
     grind
-
-theorem CoInd.le.antisymm [Inhabited (F PUnit)] c1 c2:
-  CoInd.le F c1 c2 →
-  CoInd.le F c2 c1 →
-  c1 = c2 := by
-    intro h1 h2
+  rel_antisymm := by
+    intro c1 c2 h1 h2
     ext n
     induction n generalizing c1 c2 h1 h2; rfl
     unfold CoInd.le at h1 h2
@@ -306,21 +304,12 @@ theorem CoInd.le.antisymm [Inhabited (F PUnit)] c1 c2:
     simp [QPF.map, *]
     grind
 
-open Lean.Order
-open Classical
-
-instance [Inhabited (F PUnit)] : PartialOrder (CoInd F) where
-  rel := CoInd.le F
-  rel_refl := CoInd.le.rfl F _
-  rel_trans := CoInd.le.trans F _ _ _
-  rel_antisymm := CoInd.le.antisymm F _ _
-
 noncomputable def CoInd.csup [Inhabited (F PUnit)] (c : CoInd F → Prop) : CoInd F :=
   cofix F (λ c =>
-    if h : ∃ t, c t ∧ t ≠ CoInd.le.bot F then
+    if h : ∃ t, c t ∧ t ≠ CoInd.bot F then
       let .obj i _ := QPF.unpack (choose h).unfold;
       QPF.pack $ .obj i λ o c' =>
-        ∃ c0, c c0 ∧ c0 ≠ CoInd.le.bot F ∧
+        ∃ c0, c c0 ∧ c0 ≠ CoInd.bot F ∧
           let .obj i' k := QPF.unpack c0.unfold
           ∃ eq : i = i', c' = k (cast (congrArg _ eq) o)
     else
@@ -328,10 +317,10 @@ noncomputable def CoInd.csup [Inhabited (F PUnit)] (c : CoInd F → Prop) : CoIn
   ) c
 
 theorem CoInd.csup_eq [Inhabited (F PUnit)] (c : CoInd F → Prop) :
-  csup F c = if h : ∃ t, c t ∧ t ≠ CoInd.le.bot F then
+  csup F c = if h : ∃ t, c t ∧ t ≠ CoInd.bot F then
       let .obj i _ := QPF.unpack (choose h).unfold
       CoInd.fold F $ QPF.pack $ .obj i λ o => csup F λ c' =>
-        ∃ c0, c c0 ∧ c0 ≠ CoInd.le.bot F ∧
+        ∃ c0, c c0 ∧ c0 ≠ CoInd.bot F ∧
          let .obj i' k := QPF.unpack c0.unfold
          ∃ eq : i = i', c' = k (cast (congrArg _ eq) o)
     else
@@ -341,27 +330,30 @@ theorem CoInd.csup_eq [Inhabited (F PUnit)] (c : CoInd F → Prop) :
   repeat split <;> simp
 
 theorem CoInd.csup_eq_bot {c} [Inhabited (F PUnit)]:
-  (¬∃ t, c t ∧ t ≠ le.bot F) →
-  CoInd.csup F c = le.bot F := by
+  (¬∃ t, c t ∧ t ≠ bot F) →
+  CoInd.csup F c = bot F := by
     intro h
     ext n
     induction n; rfl
     next n ih =>
-    rw [CoInd.le.bot_eq, CoInd.csup_eq]
+    rw [CoInd.bot_eq, CoInd.csup_eq]
     simp [*, fold_approx]
+
+theorem CoInd.le_unfold [Inhabited (F PUnit)] c1 c2 :
+  (c1 ⊑ c2) = (c1 = bot F ∨ coherent1 (PartialOrder.rel) (QPF.unpack c1.unfold) (QPF.unpack c2.unfold)) := by simp [PartialOrder.rel, CoInd.le]
 
 theorem CoInd.le_chain_step [Inhabited (F PUnit)] c c1 c2 i1 k1 i2 k2:
   c c1 →
   c c2 →
   chain c →
-  c1 ≠ le.bot F →
-  c2 ≠ le.bot F →
+  c1 ≠ bot F →
+  c2 ≠ bot F →
   QPF.unpack (unfold F c1) = .obj i1 k1 →
   QPF.unpack (unfold F c2) = .obj i2 k2 →
   ∃ eq : i1 = i2, (∀ o, k1 o ⊑ k2 (cast (congrArg _ eq) o) ∨ k2 (cast (congrArg _ eq) o) ⊑ k1 o) := by
     intros _ _ hc _ _ _ _
     obtain h | h := hc c1 c2 (by assumption) (by assumption)
-    . simp [PartialOrder.rel, CoInd.le, *] at h
+    . simp [CoInd.le_unfold, *] at h
       cases h
       simp_all
       rename (_ ∧ _) => h
@@ -370,9 +362,8 @@ theorem CoInd.le_chain_step [Inhabited (F PUnit)] c c1 c2 i1 k1 i2 k2:
       rename (_ ∧ _) => h
       cases h
       subst_eqs
-      simp [PartialOrder.rel]
       grind
-    . simp [PartialOrder.rel, CoInd.le, *] at h
+    . simp [CoInd.le_unfold, *] at h
       cases h
       simp_all
       rename (_ ∧ _) => h
@@ -381,16 +372,15 @@ theorem CoInd.le_chain_step [Inhabited (F PUnit)] c c1 c2 i1 k1 i2 k2:
       rename (_ ∧ _) => h
       cases h
       subst_eqs
-      simp [PartialOrder.rel]
       grind
 
 theorem CoInd.csup_step {c} [Inhabited (F PUnit)] t i k:
   c t →
   chain c →
-  t ≠ le.bot F →
+  t ≠ bot F →
   QPF.unpack t.unfold = .obj i k →
   CoInd.csup F c = CoInd.fold F (QPF.pack $ .obj i
-    λ o => CoInd.csup F λ c' => ∃ c0, c c0 ∧ c0 ≠ CoInd.le.bot F ∧
+    λ o => CoInd.csup F λ c' => ∃ c0, c c0 ∧ c0 ≠ CoInd.bot F ∧
         let .obj i' k := QPF.unpack c0.unfold
         ∃ eq : i = i', c' = k (cast (congrArg _ eq) o)) := by
     intro ht hc _ _
@@ -410,11 +400,11 @@ theorem CoInd.csup_spec [Inhabited (F PUnit)] {c : CoInd F → Prop}
   intro x
   constructor
   · intro hsup t ht
-    apply CoInd.le.trans; rotate_left 1; assumption
+    apply PartialOrder.rel_trans; rotate_left 1; assumption
     apply le.coinduct _ (λ c1 c2 => ∃ c, c c1 ∧ chain c ∧ c2 = csup F c); rotate_left 1; grind
     rintro c1 c2 ⟨c, hc1, hc, heq⟩
     subst_eqs
-    by_cases (c1 = le.bot F)
+    by_cases (c1 = bot F)
     . grind
     right
     rcases h : (QPF.unpack (unfold F c1)); rotate_left 1; trivial
@@ -431,7 +421,7 @@ theorem CoInd.csup_spec [Inhabited (F PUnit)] {c : CoInd F → Prop}
     apply le.coinduct _ (λ c1 c2 => ∃ c, chain c ∧ c1 = csup F c ∧ (∀ (y : CoInd F), c y → y ⊑ c2)); rotate_left 1; grind
     rintro c1 c2 ⟨c, hc, heq, hc2⟩
     subst_eqs
-    by_cases h : ∃ t, c t ∧ t ≠ CoInd.le.bot F
+    by_cases h : ∃ t, c t ∧ t ≠ CoInd.bot F
     . right
       rcases h with ⟨t, _, _⟩
       cases h : (QPF.unpack (unfold F t)) <;> try trivial
@@ -439,7 +429,8 @@ theorem CoInd.csup_spec [Inhabited (F PUnit)] {c : CoInd F → Prop}
       cases h2 : (QPF.unpack (unfold F c2)) <;> try trivial
       simp
       have heq := hc2 t (by assumption)
-      simp [PartialOrder.rel, le, *] at heq
+      rw [CoInd.le_unfold] at heq
+      simp [*] at heq
       rcases heq
       simp_all
       rename (_ ∧ _) => h
@@ -458,13 +449,13 @@ theorem CoInd.csup_spec [Inhabited (F PUnit)] {c : CoInd F → Prop}
         subst_eqs
         simp
         have heq := hc2 c' (by assumption)
-        simp [PartialOrder.rel, le, *] at heq
+        rw [CoInd.le_unfold] at heq
+        simp [*] at heq
         rcases heq
         simp_all
         rename (_ ∧ _) => h
         cases h
         subst_eqs
-        simp [PartialOrder.rel]
         grind
       rintro x y ⟨c1, _, _, hm1⟩ ⟨c2, _, _, hm2⟩
       grind [CoInd.le_chain_step]
@@ -472,3 +463,141 @@ theorem CoInd.csup_spec [Inhabited (F PUnit)] {c : CoInd F → Prop}
 
 noncomputable instance (priority := default + 100) [Inhabited (F PUnit)] : CCPO (CoInd F) where
   has_csup {c} ch := .intro (CoInd.csup F c) (CoInd.csup_spec F ch)
+
+section CoIndN_le
+
+theorem coherent_unfold_eq_i (x : CoInd F) n {i1 k1 i2 k2}:
+  QPF.unpack (x.approx (n + 1)) = .obj i1 k1 →
+  QPF.unpack (x.unfold) = .obj i2 k2 →
+  i1 = i2 := by
+    simp [CoInd.unfold]
+    split
+    simp
+    grind [coherent_eq_i]
+
+theorem coherent_unfold_eq_k (x : CoInd F) n {i k1 k2} o:
+  QPF.unpack (x.approx (n + 1)) = .obj i k1 →
+  QPF.unpack (x.unfold) = .obj i k2 →
+  k1 o = (k2 o).approx n := by
+    simp [CoInd.unfold]
+    split
+    simp
+    rintro _ rfl rfl
+    simp
+    split
+    simp_all
+    rename (_ ∧ _) => h
+    cases h
+    subst_eqs
+    simp
+
+def CoIndN.bot [Inhabited (F PUnit)] (n : Nat) : CoIndN F n :=
+  (CoInd.bot F).approx n
+
+theorem CoIndN.bot.eq_plus_1 [Inhabited (F PUnit)] n:
+  CoIndN.bot F (n + 1) = QPF.map F (λ _ : PUnit => CoIndN.bot F n) default := by
+    unfold CoIndN.bot
+    rw (occs:=[1]) [CoInd.bot_eq]
+    simp [CoInd.fold]
+
+def CoIndN.le {n} [Inhabited (F PUnit)] (c1 : CoIndN F n) (c2 : CoIndN F n) : Prop :=
+  match n with
+  | 0 => True
+  | n+1 => c1 = bot F (n+1) ∨ coherent1 CoIndN.le (QPF.unpack c1) (QPF.unpack c2)
+coinductive_fixpoint monotonicity fun f f' himp => by
+  rintro ⟨_|_⟩ _ _ h <;> simp at *
+  cases h
+  · grind
+  next h =>
+  right; cases h; constructor <;> try assumption
+  intro _; apply himp; grind
+
+theorem CoInd.le_leN [Inhabited (F PUnit)] (c1 c2 : CoInd F) :
+  (∀ n, CoIndN.le F (c1.approx n) (c2.approx n)) →
+  c1 ⊑ c2 := by
+    intro hn;  apply CoInd.le.coinduct _ (λ c1 c2 => (∀ n, CoIndN.le F (c1.approx n) (c2.approx n)))
+    rotate_right 1; grind
+    intro c1 c2 ih
+    by_cases hbot : (c1 = CoInd.bot F); grind
+    right
+    by_cases hex : (∃ n, c1.approx n ≠ CoIndN.bot F n)
+    · rcases hex with ⟨n, hn⟩
+      cases n; contradiction
+      next n =>
+      have h := ih (n+1)
+      simp [CoIndN.le] at h
+      cases h; grind
+      next h =>
+      cases h
+      cases h1 : (QPF.unpack (CoInd.unfold F c1))
+      cases h2 : (QPF.unpack (CoInd.unfold F c2))
+      have := coherent_unfold_eq_i F c1 n (by assumption) (by assumption)
+      have := coherent_unfold_eq_i F c2 n (by assumption) (by assumption)
+      subst_eqs
+      constructor <;> try rfl
+      rotate_left 1
+      · rename Empty => h; cases h
+      · rename Empty => h; cases h
+      intro o m
+      have h := ih (m + 1)
+      simp [CoIndN.le] at h
+      cases h
+      · cases _ : (QPF.unpack $ c1.approx (m + 1))
+        rotate_left 1
+        · rename Empty => h; cases h
+        have := coherent_unfold_eq_i F c1 m (by assumption) (by assumption)
+        subst_eqs
+        have hk := coherent_unfold_eq_k F c1 m o (by assumption) (by assumption)
+        rw [<-hk]
+        clear hk
+        simp_all [CoIndN.bot.eq_plus_1]
+        split at *
+        simp_all
+        rename (_ ∧ _) => h
+        cases h
+        subst_eqs
+        cases m <;> simp [CoIndN.le]
+      next h =>
+      cases h
+      have := coherent_eq_i F c1 n m (by assumption) (by assumption)
+      subst_eqs
+      have := coherent_unfold_eq_k F c1 m o (by assumption) (by assumption)
+      have := coherent_unfold_eq_k F c2 m o (by assumption) (by assumption)
+      grind
+    · false_or_by_contra
+      apply hbot
+      ext n
+      false_or_by_contra
+      next h =>
+      apply hex
+      exists n
+
+theorem CoInd.leN_le [Inhabited (F PUnit)] (c1 c2 : CoInd F) n :
+  c1 ⊑ c2 →
+  CoIndN.le F (c1.approx n) (c2.approx n) := by
+    induction n generalizing c1 c2 <;> simp [CoIndN.le]
+    next n ih =>
+    intro hc
+    rw [CoInd.le_unfold] at hc
+    cases hc
+    · simp_all [CoIndN.bot]
+    next h =>
+    cases h
+    right
+    cases _ : (QPF.unpack $ c1.approx (n + 1))
+    rotate_left 1
+    · rename Empty => h; cases h
+    cases _ : (QPF.unpack $ c2.approx (n + 1))
+    rotate_left 1
+    · rename Empty => h; cases h
+    have := coherent_unfold_eq_i F c1 n (by assumption) (by assumption)
+    have := coherent_unfold_eq_i F c2 n (by assumption) (by assumption)
+    subst_eqs
+    constructor <;> try rfl
+    intro o
+    have := coherent_unfold_eq_k F c1 n o (by assumption) (by assumption)
+    have := coherent_unfold_eq_k F c2 n o (by assumption) (by assumption)
+    grind
+
+end CoIndN_le
+end partial_order
