ITree/Effects/Fail.lean
@@ -16,3 +16,12 @@ export FailE (fail)
 def failEH : SEHandler failE PUnit where
   handle i s p := True
   handle_mono := by grind
+
+theorem exec_fail {α : Type u} {GE : Effect.{u}} {GR σ p q s}
+    {k : α → ITree GE GR}
+    [failE -< GE] (eh : EHandler GE GE GR σ) [hin : InEH failEH.toEHandler eh]
+    : exec eh (fail q >>= k) s p := by
+  unfold fail
+  simp only [bind_assoc]
+  apply exec.trigger failEH.toEHandler
+  simp [failEH]
