Test/HeapLang.lean
@@ -1,0 +1,422 @@
+import Lean.PrettyPrinter.Delaborator
+import ITree
+
+open ITree
+open ITree.Effects
+open ITree.Exec
+
+namespace HeapLang
+
+@[ext]
+structure Loc where
+  private mk ::
+  private n : Int
+deriving Inhabited, Repr, DecidableEq
+
+instance : Ord Loc where
+  compare l₁ l₂ := compare l₁.n l₂.n
+
+instance : Std.TransOrd Loc where
+  eq_swap := by
+    intros l₁ l₂; unfold compare; unfold instOrdLoc; simp;
+    apply Int.instTransOrd.eq_swap
+  isLE_trans := by
+    intros l₁ l₂ l₃; unfold compare; unfold instOrdLoc; simp;
+    apply Int.instTransOrd.isLE_trans
+
+instance : Std.LawfulEqOrd Loc where
+  eq_of_compare := by
+    intros l₁ l₂; unfold compare; unfold instOrdLoc; simp;
+    intros h; ext; assumption
+
+def Loc.offset (l : Loc) (i : Int) : Loc := ⟨l.n + i⟩
+
+@[ext]
+structure ProphId where
+  private mk ::
+  private n : Nat
+deriving Inhabited, Repr, DecidableEq
+
+inductive Binder where
+  | anon
+  | named (name : String)
+deriving Inhabited, Repr, DecidableEq
+
+inductive BaseLit where
+  | int (n : Int)
+  | bool (b : Bool)
+  | unit
+  | poison
+  | loc (l : Loc)
+  | prophecy (p : ProphId)
+deriving Inhabited, Repr, DecidableEq
+
+inductive UnOp where
+  | neg
+  | minus
+deriving Inhabited, Repr, DecidableEq
+
+inductive BinOp where
+  /- We use "tdiv" and "tmod" instead of "div" and "mod" to
+      better match the behavior of 'real' languages:
+      e.g., in Rust, -30 / -4 == 7. ("div" would return 8.) -/
+  | plus | minus | mult | tdiv | tmod /- arithmetic -/
+  | and | or | xor /- bitwise -/
+  | shiftl | shiftr /- shifts -/
+  | le | lt | eq /- relations -/
+  | offset /- pointer offset -/
+deriving Inhabited, Repr, DecidableEq
+
+mutual
+  inductive Exp : Type where
+    /- values -/
+    | val (v : Val)
+    /- Base lambda calculus -/
+    | var (x : String)
+    | rec_ (f x : Binder) (e : Exp)
+    | app (e₁ e₂ : Exp)
+    /- Base types and their operations -/
+    | unop (op : UnOp) (e : Exp)
+    | binop (op : BinOp) (e₁ e₂ : Exp)
+    | if (e₀ e₁ e₂ : Exp)
+    /- Products -/
+    | pair (e₁ e₂ : Exp)
+    | fst (e : Exp)
+    | snd (e : Exp)
+    /- Sums -/
+    | injL (e : Exp)
+    | injR (e : Exp)
+    | case (e₀ e₁ e₂ : Exp)
+    /- Heap -/
+    | allocN (e₁ e₂ : Exp) /- array length, initial value -/
+    | free (e : Exp)
+    | load (e : Exp)
+    | store (e₁ e₂ : Exp)
+    | cmpXchg (e₀ e₁ e₂ : Exp) /- compare exchange -/
+    | xchg (e₁ e₂ : Exp) /- exchange -/
+    | faa (e₁ e₂ : Exp) /- fetch and add -/
+    /- Concurrency -/
+    | fork (e : Exp)
+    /- Prophecy -/
+    | newProph
+    | resolve (e₀ e₁ e₂ : Exp)
+  deriving Inhabited, Repr, DecidableEq
+  inductive Val : Type where
+    | lit (l : BaseLit)
+    | rec_ (f x : Binder) (e : Exp)
+    | pair (v₁ v₂ : Val)
+    | injL (v : Val)
+    | injR (v : Val)
+  deriving Inhabited, Repr, DecidableEq
+end
+
+def Exp.isVal : Exp → Bool
+  | .val _ => true
+  | _ => false
+
+instance : Coe Nat Val where
+  coe n := .lit $ .int n
+
+instance : Coe Int Val where
+  coe n := .lit $ .int n
+
+instance : Coe Unit Val where
+  coe _ := .lit $ .unit
+
+instance {n} : OfNat Val n where
+  ofNat := .lit $ .int n
+
+def Exp.substStr (x : String) (v : Val) (e : Exp) : Exp :=
+  match e with
+  | .val _ => e
+  | .var x' => if x == x' then .val v else e
+  | .rec_ f x' e => .rec_ f x' $ if .named x != f && .named x != x' then e.substStr x v else e
+  | .app e₁ e₂ => .app (e₁.substStr x v) (e₂.substStr x v)
+  | .unop op e' => .unop op (e'.substStr x v)
+  | .binop op e₁ e₂ => .binop op (e₁.substStr x v) (e₂.substStr x v)
+  | .if e₀ e₁ e₂ => .if (e₀.substStr x v) (e₁.substStr x v) (e₂.substStr x v)
+  | .pair e₁ e₂ => .pair (e₁.substStr x v) (e₂.substStr x v)
+  | .fst e' => .fst (e'.substStr x v)
+  | .snd e' => .snd (e'.substStr x v)
+  | .injL e' => .injL (e'.substStr x v)
+  | .injR e' => .injR (e'.substStr x v)
+  | .case e₀ e₁ e₂ => .case (e₀.substStr x v) (e₁.substStr x v) (e₂.substStr x v)
+  | .allocN e₁ e₂ => .allocN (e₁.substStr x v) (e₂.substStr x v)
+  | .free e' => .free (e'.substStr x v)
+  | .load e' => .load (e'.substStr x v)
+  | .store e₁ e₂ => .store (e₁.substStr x v) (e₂.substStr x v)
+  | .cmpXchg e₀ e₁ e₂ => .cmpXchg (e₀.substStr x v) (e₁.substStr x v) (e₂.substStr x v)
+  | .xchg e₁ e₂ => .xchg (e₁.substStr x v) (e₂.substStr x v)
+  | .faa e₁ e₂ => .faa (e₁.substStr x v) (e₂.substStr x v)
+  | .fork e' => .fork (e'.substStr x v)
+  | .newProph => .newProph
+  | .resolve e₀ e₁ e₂ => .resolve (e₀.substStr x v) (e₁.substStr x v) (e₂.substStr x v)
+
+def Exp.subst (x : Binder) (v : Val) (e : Exp) : Exp :=
+  if let .named x := x then Exp.substStr x v e else e
+
+def BaseLit.isUnboxed : BaseLit → Bool
+  | .prophecy _ | .poison => false
+  | _ => true
+
+def Val.isUnboxed : Val → Bool
+  | .lit l => l.isUnboxed
+  | .injL (.lit l) => l.isUnboxed
+  | .injR (.lit l) => l.isUnboxed
+  | _ => false
+
+def Val.int! [failE -< E] : Val → ITree E Int
+  | .lit (.int i) => return i
+  | x => fail s!"{reprStr x} is not Int"
+
+def Val.bool! [failE -< E] : Val → ITree E Bool
+  | .lit (.bool b) => return b
+  | x => fail s!"{reprStr x} is not Bool"
+
+def Val.loc! [failE -< E] : Val → ITree E Loc
+  | .lit (.loc l) => return l
+  | x => fail s!"{reprStr x} is not Loc"
+
+def Val.pair! [failE -< E] : Val → ITree E (Val × Val)
+  | .pair v1 v2 => return (v1, v2)
+  | x => fail s!"{reprStr x} is not Pair"
+
+def Val.rec! [failE -< E] : Val → ITree E (Binder × Binder × Exp)
+  | .rec_ f x e => return (f, x, e)
+  | x => fail s!"{reprStr x} is not Rec"
+
+def Val.injL! [failE -< E] : Val → ITree E Val
+  | .injL v => return v
+  | x => fail s!"{reprStr x} is not InjL"
+
+def Val.injR! [failE -< E] : Val → ITree E Val
+  | .injR v => return v
+  | x => fail s!"{reprStr x} is not InjR"
+
+abbrev heaplangE := concE ⊕ₑ heapE Loc Val ⊕ₑ failE ⊕ₑ demonicE (List Loc)
+def heaplangEH {GE GR} := concEH (GE:=GE) (GR:=GR) ⊕ₑₕ (heapEH Loc Val ⊕ₛₑₕ failEH ⊕ₛₑₕ demonicEH (List Loc)).toEHandler
+
+instance {GE GR GR'} : EHandlerBind (GE:=GE) (GR:=GR) (GR':=GR')
+  heaplangEH (failingEH ⊕ₑₕ (heapEH Loc Val ⊕ₛₑₕ failEH ⊕ₛₑₕ demonicEH (List Loc)).toEHandler) := inferInstanceAs (EHandlerBind (concEH ⊕ₑₕ _) _)
+
+def UnOp.denote (op : UnOp) (v : Val) : ITree heaplangE Val :=
+  match op, v with
+  | .neg, .lit (.bool b) => return .lit (.bool !b)
+  | .neg, .lit (.int n) => return .lit (.int (~~~n))
+  | .minus, .lit (.int n) => return .lit (.int (-n))
+  | _, _ => fail "UnOp: type mismatch"
+
+def BinOp.evalInt (op : BinOp) (n₁ n₂ : Int) : Option BaseLit :=
+  match op with
+  | .plus => some $ .int (n₁ + n₂)
+  | .minus => some $ .int (n₁ - n₂)
+  | .mult => some $ .int (n₁ * n₂)
+  | .tdiv => some $ .int (Int.tdiv n₁ n₂)
+  | .tmod => some $ .int (Int.tmod n₁ n₂)
+/- TODO: get rid of the toNat and define the operations directly on Int -/
+  | .and => some $ .int (Nat.land n₁.toNat n₂.toNat : Nat)
+  | .or => some $ .int (Nat.lor n₁.toNat n₂.toNat : Nat)
+  | .xor => some $ .int (Nat.xor n₁.toNat n₂.toNat : Nat)
+  | .shiftl => some $ .int (n₁ <<< n₂.toNat)
+  | .shiftr => some $ .int (n₁ >>> n₂.toNat)
+  | .le => some $ .bool (decide (n₁ ≤ n₂))
+  | .lt => some $ .bool (decide (n₁ < n₂))
+  | .eq => some $ .bool (decide (n₁ = n₂))
+  | .offset => none
+
+def BinOp.evalBool (op : BinOp) (b₁ b₂ : Bool) : Option BaseLit :=
+  match op with
+  | .and => some $ .bool (b₁ && b₂)
+  | .or => some $ .bool (b₁ || b₂)
+  | .xor => some $ .bool (Bool.xor b₁ b₂)
+  | .eq => some $ .bool (decide (b₁ = b₂))
+  | _ => none
+
+def BinOp.evalLoc (op : BinOp) (l₁ : Loc) (v₂ : BaseLit) : Option BaseLit :=
+  match op, v₂ with
+  | .offset, .int off => some $ .loc (l₁.offset off)
+  | .le, .loc l₂ => some $ .bool (decide (l₁.n ≤ l₂.n))
+  | .lt, .loc l₂ => some $ .bool (decide (l₁.n < l₂.n))
+  | _, _ => none
+
+def BinOp.denote (op : BinOp) (v₁ v₂ : Val) : ITree heaplangE Val :=
+  if op == .eq then
+    if v₁.isUnboxed || v₂.isUnboxed then
+      return .lit (.bool (decide (v₁ = v₂)))
+    else
+      fail "EqOp: comparing boxed values"
+  else
+    match v₁, v₂ with
+    | .lit (.int n₁), .lit (.int n₂) => do
+      let .some l := BinOp.evalInt op n₁ n₂
+        | fail "BinOp: invalid int operation"
+      return .lit l
+    | .lit (.bool b₁), .lit (.bool b₂) => do
+      let some l := BinOp.evalBool op b₁ b₂
+        | fail "BinOp: invalid bool operation"
+      return .lit l
+    | .lit (.loc l₁), .lit v₂ => do
+      let some l := BinOp.evalLoc op l₁ v₂
+        | fail "BinOp: invalid loc operation"
+      return .lit l
+    | _, _ => fail "BinOp: type mismatch"
+
+def Exp.yieldIfNotVal : Exp → ITree heaplangE Unit
+  | .val _ => return ()
+  | _ => yield
+
+/- TODO: check all the yields and add step -/
+def Exp.denote (e : Exp) : ITree heaplangE Val :=
+  let denoteYield e :=
+    if e.isVal then denote e else yieldAfter (denote e)
+  match e with
+  | .val v => return v
+  | .var x => fail s!"Unbound variable {reprStr x}"
+  | .rec_ f x e => return .rec_ f x e
+  | .app e₁ e₂ => do
+    let v ← denoteYield e₂
+    let f ← denoteYield e₁
+    let ⟨f', x', e⟩ ← f.rec!
+    let body := e.subst f' f |>.subst x' v
+    body.yieldIfNotVal
+    denote body
+  | .unop op e => do
+    let v ← denoteYield e
+    op.denote v
+  | .binop op e₁ e₂ => do
+    let v₂ ← denoteYield e₂
+    let v₁ ← denoteYield e₁
+    op.denote v₁ v₂
+  | .if e₀ e₁ e₂ => do
+    let c ← denoteYield e₀
+    if ← c.bool! then
+      denoteYield e₁
+    else
+      denoteYield e₂
+  | .pair e₁ e₂ => do
+    let v₂ ← denoteYield e₂
+    let v₁ ← denoteYield e₁
+    return .pair v₁ v₂
+  | .fst e => do
+    let v ← denoteYield e
+    return (← v.pair!).1
+  | .snd e => do
+    let v ← denoteYield e
+    return (← v.pair!).2
+  | .injL e => do
+    let v ← denoteYield e
+    return .injL v
+  | .injR e => do
+    let v ← denoteYield e
+    return .injR v
+  | .case e₀ e₁ e₂ => do
+    let v ← denoteYield e₀
+    match v with
+    | .injL w => yield; denote (.app e₁ (.val w))
+    | .injR w => yield; denote (.app e₂ (.val w))
+    | _ => fail "Case: not a sum value"
+  | .allocN e₁ e₂ => do
+    let v ← denoteYield e₂
+    let vn ← denoteYield e₁
+    let n ← vn.int!
+    if n ≤ 0 then fail "AllocN: count must be positive"
+    let ⟨ls, _⟩ ← HeapE.allocN (λ ls => ∃ l : Loc, ls = (List.range n.toNat).map λ n => l.offset (Int.ofNat n)) v
+    return .lit (.loc ls.head!)
+  | .free e => do
+    let v ← denoteYield e
+    let l ← v.loc!
+    let .some _ ← storeOpt (Val:=Val) l none
+      | fail "free: location not allocated"
+    return .lit .unit
+  | .load e => do
+    let v ← denoteYield e
+    load! (← v.loc!)
+  | .store e₁ e₂ => do
+    let v₂ ← denoteYield e₂
+    let v₁ ← denoteYield e₁
+    let _ ← store! (← v₁.loc!) v₂
+    return .lit .unit
+  | .cmpXchg e₀ e₁ e₂ => do
+    let v₂ ← denoteYield e₂
+    let v₁ ← denoteYield e₁
+    let v₀ ← denoteYield e₀
+    let l ← v₀.loc!
+    let vl ← load! l
+    if !(vl.isUnboxed || v₁.isUnboxed) then
+      fail "CmpXchg: comparing boxed values"
+    if vl = v₁ then
+      let _ ← store! l v₂
+      return .pair vl (.lit (.bool true))
+    else
+      return .pair vl (.lit (.bool false))
+  | .xchg e₁ e₂ => do
+    let v₂ ← denoteYield e₂
+    let v₁ ← denoteYield e₁
+    store! (← v₁.loc!) v₂
+  | .faa e₁ e₂ => do
+    let v₂ ← denoteYield e₂
+    let v₁ ← denoteYield e₁
+    let l ← v₁.loc!
+    let i₂ ← v₂.int!
+    let old ← load! l
+    let i₁ ← old.int!
+    let _ ← store! l (.lit (.int (i₁ + i₂)) : Val)
+    return old
+  | .fork e => do
+    let _ ← ConcE.fork (denoteYield e >>= λ _ => return ⟨⟩)
+    return .lit .unit
+  | .newProph => do
+    fail "prophecy is not implemented"
+  | .resolve _ _ _ => do
+    fail "prophecy is not implemented"
+partial_fixpoint
+
+section Notation
+open Lean Lean.PrettyPrinter Elab Parser
+
+declare_syntax_cat hl_exp
+-- declare_syntax_cat hl_val
+
+syntax:max "hl(" hl_exp ")" : term
+-- syntax:max "hl_val(" hl_val ")" : term
+syntax:max "{" term "}" : hl_exp
+syntax:max "#" term:max : hl_exp
+-- syntax:max "#" term:max : hl_val
+syntax:65 hl_exp:66 " + " hl_exp:65 : hl_exp
+
+macro_rules
+  | `(hl({$t})) => pure t
+  | `(hl($e1 + $e2)) => `(Exp.binop .plus hl($e1) hl($e2))
+  | `(hl(# $e)) => `(Exp.val $e)
+  -- | `(hl(# $e)) => `(Exp.val hl_val(#$e))
+  -- | `(hl_val(# $e)) => `(Val.lit $e)
+
+
+-- @[app_unexpander Val.lit]
+-- def unexpLit : Unexpander
+  -- | `($_ $arg) => `(hl_val(# $arg))
+  -- | _ => throw ()
+
+-- @[app_unexpander Exp.val]
+-- def unexpVal : Unexpander
+--   | `($_ hl_val(# $arg)) => `(hl(# $arg))
+--   | _ => throw ()
+
+@[app_unexpander Exp.val]
+def unexpVal : Unexpander
+  | `($_ $arg) => `(hl(# $arg))
+  | _ => throw ()
+
+partial def unpackHLExp [Monad m] [MonadRef m] [MonadQuotation m] : Term → m (TSyntax `hl_exp)
+  | `(hl($e)) => `(hl_exp|$e)
+  | `($t) => `(hl_exp|{$t})
+
+
+@[app_unexpander Exp.binop]
+def unexpBinop : Unexpander
+  | `($_ BinOp.plus $e1 $e2) => do `(hl($(← unpackHLExp e1) + $(← unpackHLExp e2)))
+  | _ => throw ()
+
+variable (v : Val)
+#check hl(#1 + #1 + {.val v})
+#check hl(#1 + #1 + #v)
