Test/HeapLangExamples.lean
@@ -1,0 +1,17 @@
+import Test.HeapLang
+
+open ITree
+open ITree.Effects
+open ITree.Exec
+
+namespace HeapLang
+
+example s :
+  exec heaplangEH (Exp.denote (.binop .plus (.val 1) (.val 1))) s λ t _ => t = return (.lit $ .int 2) := by
+    simp [Exp.denote, Exp.isVal, BinOp.denote, BinOp.evalInt]
+    -- apply exec.bind
+    -- simp [Val.int!]
+    -- apply exec.stop
+    -- simp
+    apply exec.stop
+    simp
