Test/Stream.lean
@@ -30,19 +30,81 @@ def Stream.fold (t : StreamF α (Stream α)) : Stream α := CoInd.fold _ t
 def Stream.snil {α : Type u} : Stream α := Stream.fold (.snil)
 def Stream.scons {α : Type u} (hd : α) (tl : Stream α) : Stream α := Stream.fold (.scons hd tl)
 
+@[simp]
+theorem snil_approx_1 α n :
+  (Stream.snil (α:=α)).approx (n + 1) = StreamF.snil := by
+    simp [Stream.snil, Stream.fold, CoInd.fold, QPF.map, QPF.pack]
+
+@[simp]
+theorem scons_approx_1 α i (s : Stream α) n :
+  (Stream.scons i s).approx (n + 1) = StreamF.scons i (s.approx n) := by
+    simp [Stream.scons, Stream.fold, CoInd.fold, QPF.map, QPF.pack]
+
+@[simp]
+theorem unfold_snil α :
+  CoInd.unfold _ Stream.snil = StreamF.snil (α:=α) := by
+    simp [Stream.snil, Stream.fold]
+
+@[simp]
+theorem unfold_scons α (i : α) s:
+  CoInd.unfold _ (Stream.scons i s) = StreamF.scons i s := by
+    simp [Stream.scons, Stream.fold]
+
 instance : Inhabited (StreamF α PUnit) where default := .snil
+
+@[simp]
+theorem Stream.bot_eq α :
+  CoInd.bot (StreamF α) = Stream.snil := by
+    rw [CoInd.bot_eq]
+    simp [QPF.map, QPF.pack, Stream.snil, Stream.fold]
+
+
+theorem Stream.le_unfold α (s1 s2 : Stream α) :
+  (s1 ⊑ s2) = (s1 = .snil ∨
+    ∃ i s1' s2', s1 = .scons i s1' ∧ s2 = .scons i s2' ∧ s1' ⊑ s2') := by
+    ext
+    constructor
+    · intro h
+      rw [CoInd.le_unfold] at h
+      rcases h with (rfl|⟨i, _, _, _, _, h1, h2⟩); simp
+      rw [<-unfold_fold _ s1, <-unfold_fold _ s2]
+      rw [<-QPF.unpack_pack s1.unfold, <-QPF.unpack_pack s2.unfold]
+      simp only [h1, h2]
+      cases i <;> simp [QPF.pack, snil, scons, fold]
+      right
+      exists ?_, ?_; rotate_left 1
+      constructor; rfl
+      apply Exists.intro
+      constructor; rfl
+      simp_all
+    · rintro (rfl|⟨_, _, _, rfl, rfl, _⟩)
+      · simp [CoInd.le_unfold]
+      · simp [CoInd.le_unfold]
+        right
+        simp [QPF.unpack]
+        constructor <;> try rfl
+        grind
+
+theorem scons_monoN α i (s1 s2 : Stream α) n :
+  CoIndN.le _ (s1.approx n) (s2.approx n) →
+  CoIndN.le _ ((Stream.scons i s1).approx (n + 1))
+    ((Stream.scons i s2).approx (n + 1))
+ := by
+    intro hs
+    simp [CoIndN.le, QPF.unpack]
+    right
+    constructor <;> try rfl
+    grind [coherent1]
 
 @[partial_fixpoint_monotone]
 theorem scons_mono β α [PartialOrder β] i (f : β → Stream α) :
   monotone f →
   monotone (λ x => Stream.scons i (f x)) := by
     intro hf t1 t2 hle
-    simp [PartialOrder.rel, CoInd.le, QPF.unpack]
-    right
-    constructor <;> try rfl
-    intro _
-    apply hf
-    apply hle
+    apply CoInd.le_leN
+    rintro ⟨n⟩; simp [CoIndN.le]
+    apply scons_monoN
+    grind [CoInd.leN_le, monotone]
 
 def Stream.map {α} (f : α → β) (s : Stream α) : Stream β :=
   match s.unfold with
@@ -55,8 +117,21 @@ theorem map_mono α β γ [PartialOrder γ] (f : α → β) (g : γ → Stream �
   monotone g →
   monotone (λ x => Stream.map f (g x)) := by
     intro hf t1 t2 hle
-    simp [PartialOrder.rel, CoInd.le, QPF.unpack]
-    sorry
+    apply CoInd.le_leN
+    intro n
+    dsimp only
+    have hs : (g t1) ⊑ (g t2) := by grind [monotone]
+    generalize g t1 = s1, g t2 = s2 at hs
+    induction n generalizing s1 s2; simp [CoIndN.le]
+    unfold Stream.map
+    rw [Stream.le_unfold] at hs
+    rcases hs with ⟨_|_⟩
+    · simp [CoIndN.le, CoIndN.bot]
+    next h =>
+    rcases h with ⟨_, _, _, _, _, _⟩
+    simp [*]
+    apply scons_monoN
+    grind
 
 
 def Stream.stail {α} (s : Stream α) : Stream α :=
@@ -69,8 +144,20 @@ theorem stail_mono β α [PartialOrder β] (f : β → Stream α) :
   monotone f →
   monotone (λ x => Stream.stail (f x)) := by
     intro hf t1 t2 hle
-    simp [PartialOrder.rel, CoInd.le, QPF.unpack]
-    sorry
+    apply CoInd.le_leN
+    intro n
+    dsimp only
+    cases n; simp [CoIndN.le]
+    have hs : (f t1) ⊑ (f t2) := by grind [monotone]
+    generalize f t1 = s1, f t2 = s2 at hs
+    unfold Stream.stail
+    rw [Stream.le_unfold] at hs
+    rcases hs with ⟨_|_⟩
+    · simp [CoIndN.le, CoIndN.bot]
+    next h =>
+    rcases h with ⟨_, _, _, _, _, _⟩
+    simp [*]
+    grind [CoInd.leN_le]
 
 def s3 : Stream Nat :=
   .scons 0 $ .scons 1 $ .stail s3
